coq-osiris/theories/program_logic/handler_rules.v
@@ -264,7 +264,7 @@ Section handler_proof.
       ewp_unfold_head.
       intro_state. spec_state. iMod "He".
       destruct (π !! ι0); last done.
-      iIntros "!>" (o) "Hφ'". iSpecialize ("He" with "Hφ'").
+      iIntros "!> %φ' Hφ' %o Ho". iSpecialize ("He" with "Hφ' Ho").
       ewp_mask_elim. iMod "He" as "(He & $)".
       iModIntro. rewrite /continue.
       iApply ("IH" with "He Hsh"). }
